theories/tests/task.v
@@ -9,8 +9,6 @@ Section example.
 
   Context `{i: interrupt invs 1}.
 
-  Definition f: ident := 1.
-
   Variable l: addr.
 
   Definition f_body : expr :=
@@ -18,8 +16,8 @@ Section example.
 
   Lemma ct_spec ks:
     inv N' True%I ∗
-    l ↦ vtrue @ tybool ∗ text_interp f (Function Tvoid [] f_body)
-    ⊢ WP (create_task i f 0, ks) {{ _, True%I }}.
+    l ↦ vtrue @ tybool ∗ text_interp "f" (Function Tvoid [] f_body)
+    ⊢ WP (create_task i "f" 0, ks) {{ _, True%I }}.
   Proof.
     iIntros "[#HI [Hl Hf]]".
     iApply create_task_spec.
